DynamoDbEncryption/dafny/DynamoDbEncryption/test/DDBSupport.dfy
@@ -1,0 +1,33 @@
+include "BeaconTestFixtures.dfy"
+include "../src/DDBSupport.dfy"
+
+module TestDDBSupport {
+  import opened AwsCryptographyDynamoDbEncryptionTypes
+  import opened ComAmazonawsDynamodbTypes
+  import opened DynamoDBFilterExpr
+  import opened Wrappers
+  import opened StandardLibrary
+  import opened StandardLibrary.UInt
+  import opened BeaconTestFixtures
+  import opened DynamoDBSupport
+  import opened DynamoDbEncryptionUtil
+  import opened SearchConfigToInfo
+  import SI = SearchableEncryptionInfo
+
+  method {:test} TestAddSignedBeacons() {
+    var version := GetLotsaBeacons();
+    var src := GetLiteralSource([1,2,3,4,5], version);
+    var bv :- expect ConvertVersionWithSource(FullTableConfig, version, src);
+    var search := SI.SearchInfo([bv], 0);
+    expect search.ValidState?();
+    var newItem :- expect AddSignedBeacons(Some(search), SimpleItem);
+    assert IsValid_AttributeName("aws_dbe_v_1");
+    assert IsValid_AttributeName("JustSigned");
+    var expectedNew : DDB.AttributeMap := map[
+      "aws_dbe_v_1" := AttributeValue.S(" "),
+      "JustSigned" := AttributeValue.S("Y_1984.M_May")
+    ];
+    expect newItem == SimpleItem + expectedNew;
+  }
+
+}
